fix spec of montgomery_ladder

code/experimental/curve25519/Hacl.Spec.Curve25519.AddAndDouble.fst
@@ -4,23 +4,6 @@ open FStar.Mul
 open Lib.IntTypes
 open Spec.Curve25519
 
-let add q nq nqp1 =
-  let x_1, z_1 = q in
-  let x_2, z_2 = nq in
-  let x_3, z_3 = nqp1 in
-  let a  = x_2 +% z_2 in
-  let b  = x_2 -% z_2 in
-  let c = x_3 +% z_3 in
-  let d = x_3 -% z_3 in
-  let da = d *% a in
-  let cb = c *% b in
-  let x_3 = da +% cb in
-  let z_3 = da -% cb in
-  let x_3 = x_3 *% x_3 in
-  let z_3 = z_3 *% z_3 in
-  let z_3 = z_3 *% x_1 in
-  x_3, z_3
-
 val lemma_add:
   q:proj_point -> nq:proj_point -> nqp1:proj_point ->
   Lemma (add q nq nqp1 == snd (add_and_double q nq nqp1))
@@ -31,23 +14,12 @@ val lemma_double:
   Lemma (double nq == fst (add_and_double q nq nqp1))
 let lemma_double q nq nqp1 = ()
 
-// let cswap2 (sw:uint8) (nq:proj_point) (nqp1:proj_point) =
-//   let open Lib.RawIntTypes in
-//   if uint_to_nat sw = 1 then (nqp1, nq) else (nq, nqp1)
-
-let ladder_step1 (k:scalar) (q:proj_point) (i:nat{i < 251}) (nq, nqp1, swap) =
-  let bit = ith_bit k (253-i) in
-  let sw = swap ^. bit in
-  let nq, nqp1 = cswap2 sw nq nqp1 in
-  let nq, nqp1 = add_and_double q nq nqp1 in
-  (nq, nqp1, bit)
-
 let montgomery_ladder1_0 (k:scalar) (q:proj_point) (nq:proj_point) (nqp1:proj_point) =
   // bit 255 is 0 and bit 254 is 1
   let nq,nqp1 = cswap2 (u64 1) nq nqp1 in
   let nq,nqp1 = add_and_double q nq nqp1 in
   let swap = u64 1 in
-  let nq,nqp1,swap = Lib.LoopCombinators.repeati 251 (ladder_step1 k q) (nq, nqp1, swap) in
+  let nq,nqp1,swap = Lib.LoopCombinators.repeati 251 (ladder_step k q) (nq, nqp1, swap) in
   let nq,nqp1 = cswap2 swap nq nqp1 in
   nq
 
@@ -70,4 +42,4 @@ let montgomery_ladder1 (init:elem) (k:scalar) : Tot proj_point =
 
 val lemma_montgomery_ladder: init:elem -> k:scalar ->
   Lemma (montgomery_ladder1 init k == montgomery_ladder init k)
-let lemma_montgomery_ladder init k = admit()
+let lemma_montgomery_ladder init k = ()
